Arithmetic: update and use generic_call_sem for fsl
- misc refactorings

Arithmetic/theories/Languages/Semantics.v
@@ -63,18 +63,30 @@ Definition Forall_routines {F S T } (pgrm : @c_program F S T)
     - all variables declared before usage
     - all functions defined before called
     - well typed
+    - no duplicate functions
 *)
 Definition well_formed_pgrm (P : fsl_pgrm) :=
     forall (env : Env) (fenv: fsl_prog_fenv),
-    Forall_routines P ( fun args decls b =>
-        (* all used variables are declared *)
-        (forall v, StringSet.In v (fsl_stmt_vars b) -> v ∈ env) /\ 
-        (* all functions are defined before being called *)
-        (forall rvar fname args, 
-            @In_stmt _fsl_statement Empty_set (FCall rvar fname args) b -> 
-            StringMap.mem fname fenv.(funs) = true
-        
-        ) /\
+        True
+        /\
+
+        Forall_routines P ( fun args decls b =>
+            True
+
+        (*
+            (* all used variables are declared *)
+            (forall v, StringSet.In v (fsl_stmt_vars b) -> v ∈ env)
+            
+
+            (* all functions are defined before being called *)
+            /\ 
+            (forall rvar fname args, 
+                @In_stmt _fsl_statement Empty_set (FCall rvar fname args) b -> 
+                StringMap.mem fname fenv.(funs) = true
+            
+        *)
+        )%dom_
+        /\
         True (* fixme: well typed ? *)
-    )%dom_
+
 .
