Arithmetic/theories/Oracle.v
@@ -12,21 +12,21 @@ Module Type Oracle.
 
     Parameter get_Γᵢ : fsl_pgrm -> Γᵢ. (* static analysis *)
 
-    Parameter oracle : ℨ -> Γᵢ -> 𝐼. (* oracle *) (* using 𝓘 messes up vscoq *)
+    Parameter oracle : ℨ ⨉ Γᵢ -> 𝐼. (* oracle *) (* using 𝓘 messes up vscoq *)
 
     Parameter ϴ :  𝐼 -> 𝔗.
 
     Parameter ϴ_int_or_mpz : forall i, ϴ i = C_Int \/  ϴ i = T_Ext Mpz.
 
-    Definition get_ty : ℨ -> Γᵢ -> 𝔗 := fun t τᵢ =>  ϴ (oracle t τᵢ). (* using 𝒯 messes up vscoq *)
+    Definition get_ty : ℨ ⨉ Γᵢ -> 𝔗 := fun x => (ϴ  (oracle x)). (* using 𝒯 messes up vscoq *)
 
 
     Parameter ty_funcall_is_ty_body: 
         forall (f : fsl_prog_fenv) fname xargs (targs:list ℨ) (iargs:list 𝐼) b, 
         StringMap.find fname f.(lfuns) = Some (xargs,b) ->
         forall te,
-        List.Forall2 (fun e => eq (oracle e te)) targs iargs ->
-                    get_ty (T_Call fname targs) te = get_ty b (StringMap.add_all xargs iargs StringMap.empty).
+        List.Forall2 (fun e => eq (oracle (e,te))) targs iargs ->
+                    get_ty (T_Call fname targs, te) = get_ty (b,StringMap.add_all xargs iargs StringMap.empty).
 
 
     (* a term always fits in an mpz and only fits in a machine integer if it is in range *)
@@ -37,7 +37,7 @@ Module Type Oracle.
 
 
     Parameter type_soundness : forall env te f t z, 
-        fsl_term_sem f env t z -> fits z (get_ty t te).
+        fsl_term_sem f env t z -> fits z (get_ty (t,te)).
 
 
     (* 
@@ -47,7 +47,7 @@ Module Type Oracle.
     Parameter convergence_of_lfuns_ty : 
         forall fname (targs:list ℨ) (iargs:list 𝐼), 
         forall (typing_envs : Ensemble Γᵢ)  (fe:Γᵢ), Ensembles.In Γᵢ typing_envs fe ->
-        (exists ty te, get_ty (T_Call fname targs) te = ty) -> 
+        (exists ty te, get_ty (T_Call fname targs, te) = ty) -> 
         Finite_sets.Finite _ typing_envs
     .
 
